Change definition of binary semTriple to take similar types as the unary one (+ change reflected in all iris rules)

theories/Iris/BinaryWeakestPre.v
@@ -775,9 +775,13 @@ Module Type IrisSignatureRules2
 Section Soundness.
 
   Definition semTriple {Γ τ} (δ : CStore Γ)
-             (PRE : iProp Σ) (s : Stm Γ τ) (POST : IVal τ -> CStore Γ -> iProp Σ) : iProp Σ :=
+             (PRE : iProp Σ) (s : Stm Γ τ) (POST : Val τ -> CStore Γ -> iProp Σ) : iProp Σ :=
     PRE -∗
-      semWP2 δ δ s s (fun v1 δ1 v2 δ2 => ⌜ v1 = v2 ⌝ ∗ ⌜ δ1 = δ2 ⌝ ∗ POST v1 δ1)%I.
+    semWP2 δ δ s s (λ v1 δ1 v2 δ2, ⌜v1 = v2⌝ ∗ ⌜δ1 = δ2⌝ ∗
+                                   match v1 with
+                                   | inl v1 => POST v1 δ1
+                                   | inr m  => True%I
+                                   end)%I.
   (* always modality needed? perhaps not because sail not higher-order? *)
   Global Arguments semTriple {Γ} {τ} δ PRE%I s%exp POST%I.
 
@@ -794,7 +798,7 @@ Section Soundness.
     end.
 
   Lemma iris_rule_consequence {Γ σ} {δ : CStore Γ}
-        {P P'} {Q Q' : IVal σ -> CStore Γ -> iProp Σ} {s : Stm Γ σ} :
+        {P P'} {Q Q' : Val σ -> CStore Γ -> iProp Σ} {s : Stm Γ σ} :
         (P ⊢ P') -> (forall v δ', Q' v δ' ⊢ Q v δ') ->
         semTriple δ P' s Q' -∗ semTriple δ P s Q.
   Proof.
@@ -803,11 +807,12 @@ Section Soundness.
     - iApply "Htriple".
       now iApply PP.
     - iIntros (v1 δ1 v2 δ2) "(-> & -> & Q')".
+      case_match; auto.
       iPoseProof (QQ with "Q'") as "Q"; auto.
   Qed.
 
   Lemma iris_rule_frame {Γ σ} {δ : CStore Γ}
-        (R P : iProp Σ) (Q : IVal σ -> CStore Γ -> iProp Σ) (s : Stm Γ σ) :
+        (R P : iProp Σ) (Q : Val σ -> CStore Γ -> iProp Σ) (s : Stm Γ σ) :
         (⊢ semTriple δ P s Q -∗ semTriple δ (R ∗ P) s (fun v δ' => R ∗ Q v δ'))%I.
   Proof.
     iIntros "Htriple [HR HP]".
@@ -815,11 +820,12 @@ Section Soundness.
     iPoseProof (semWP2_frame_l with "[HR Htriple]") as "Hwp".
     { iSplitL "HR". iExact "HR". iExact "Htriple". }
     iApply (semWP2_mono with "Hwp").
-    iIntros (? ? ? ?) "($ & $ & $ & $)".
+    iIntros ([] ? ? ?) "(R & <- & $ & H)"; auto.
+    now iFrame "R H".
   Qed.
 
   Lemma iris_rule_pull {σ Γ} (δ : CStore Γ) (s : Stm Γ σ)
-        (P : iProp Σ) (Q : Prop) (R : IVal σ -> CStore Γ -> iProp Σ) :
+        (P : iProp Σ) (Q : Prop) (R : Val σ -> CStore Γ -> iProp Σ) :
         (⊢ (⌜ Q ⌝ → semTriple δ P s R) -∗ semTriple δ (P ∧ bi_pure Q) s R).
   Proof.
     iIntros "QP [P %]".
@@ -828,7 +834,7 @@ Section Soundness.
 
   Lemma iris_rule_exist {σ Γ} (δ : CStore Γ)
         (s : Stm Γ σ) {A : Type} {P : A -> iProp Σ}
-        {Q :  IVal σ -> CStore Γ -> iProp Σ} :
+        {Q : Val σ -> CStore Γ -> iProp Σ} :
         ⊢ ((∀ x, semTriple δ (P x) s Q) -∗ semTriple δ (∃ x, P x) s Q).
   Proof.
     iIntros "Htriple [% P]".
@@ -837,8 +843,8 @@ Section Soundness.
 
   Lemma iris_rule_stm_val {Γ} (δ : CStore Γ)
         {τ : Ty} {v : Val τ}
-        {P : iProp Σ} {Q : IVal τ -> CStore Γ -> iProp Σ} :
-        ⊢ ((P -∗ Q (inl v) δ)%I -∗ semTriple δ P (stm_val τ v) Q).
+        {P : iProp Σ} {Q : Val τ -> CStore Γ -> iProp Σ} :
+        ⊢ ((P -∗ Q v δ)%I -∗ semTriple δ P (stm_val τ v) Q).
   Proof.
     iIntros "PQ P".
     iApply semWP2_val_1.
@@ -848,8 +854,8 @@ Section Soundness.
 
   Lemma iris_rule_stm_exp {Γ} (δ : CStore Γ)
         {τ : Ty} {e : Exp Γ τ}
-        {P : iProp Σ} {Q : IVal τ -> CStore Γ -> iProp Σ} :
-        ⊢ ((P -∗ Q (inl (eval e δ)) δ) -∗ semTriple δ P (stm_exp e) Q).
+        {P : iProp Σ} {Q : Val τ -> CStore Γ -> iProp Σ} :
+        ⊢ ((P -∗ Q (eval e δ) δ) -∗ semTriple δ P (stm_exp e) Q).
   Proof.
     iIntros "PQ P".
     iApply semWP2_exp.
@@ -859,38 +865,31 @@ Section Soundness.
 
   Lemma iris_rule_stm_let {Γ} (δ : CStore Γ)
         (x : PVar) (σ τ : Ty) (s : Stm Γ σ) (k : Stm (Γ ▻ x∷σ) τ)
-        (P : iProp Σ) (Q : IVal σ -> CStore Γ -> iProp Σ)
-        (R : IVal τ -> CStore Γ -> iProp Σ) :
+        (P : iProp Σ) (Q : Val σ -> CStore Γ -> iProp Σ)
+        (R : Val τ -> CStore Γ -> iProp Σ) :
         ⊢ (semTriple δ P s Q -∗
-            (∀ (v : IVal σ) (δ' : CStore Γ),
-                match v with
-                | inl v' =>
-                    semTriple (env.snoc δ' (x∷σ) v') (Q v δ') k (fun v δ'' => R v (env.tail δ''))
-                | inr m  =>
-                    semTriple δ' (Q v δ') (of_ival (inr m)) (λ v δ, R v δ)
-                end) -∗
-                semTriple δ P (let: x := s in k) R).
+            (∀ (v : Val σ) (δ' : CStore Γ),
+               semTriple (env.snoc δ' (x∷σ) v) (Q v δ') k (fun v δ'' => R v (env.tail δ''))) -∗
+               semTriple δ P (let: x := s in k) R).
   Proof.
     iIntros "Hs Hk P".
     iApply semWP2_let.
     iSpecialize ("Hs" with "P").
     iApply (semWP2_mono with "Hs").
     iIntros (v1 δ1 v2 δ2) "(<- & <- & Q)".
-    iSpecialize ("Hk" $! v1 δ1).
-    destruct v1 as [v1|m1];
+    destruct v1 as [v1|m1].
+    - iSpecialize ("Hk" $! v1 δ1).
       iSpecialize ("Hk" with "Q").
-    - iApply (semWP2_mono with "Hk").
+      iApply (semWP2_mono with "Hk").
       iIntros (? ? ? ?) "(<- & <- & R)".
       by iFrame "R".
-    - iApply (semWP2_mono with "Hk").
-      iIntros (? ? ? ?) "(<- & <- & R)".
-      by iFrame "R".
+    - simpl. iApply semWP2_fail. auto.
   Qed.
 
   Lemma iris_rule_stm_block {Γ} (δ : CStore Γ)
         (Δ : PCtx) (δΔ : CStore Δ)
         (τ : Ty) (k : Stm (Γ ▻▻ Δ) τ)
-        (P : iProp Σ) (R : IVal τ -> CStore Γ -> iProp Σ) :
+        (P : iProp Σ) (R : Val τ -> CStore Γ -> iProp Σ) :
         ⊢ (semTriple (δ ►► δΔ) P k (fun v δ'' => R v (env.drop Δ δ'')) -∗
             semTriple δ P (stm_block δΔ k) R).
   Proof.
@@ -901,19 +900,21 @@ Section Soundness.
 
   Lemma iris_rule_stm_seq {Γ} (δ : CStore Γ)
         (τ : Ty) (s1 : Stm Γ τ) (σ : Ty) (s2 : Stm Γ σ)
-        (P : iProp Σ) (Q : IVal τ -> CStore Γ -> iProp Σ) (R : IVal σ -> CStore Γ -> iProp Σ) :
+        (P : iProp Σ) (Q : Val τ -> CStore Γ -> iProp Σ) (R : Val σ -> CStore Γ -> iProp Σ) :
     ⊢ semTriple δ P s1 Q -∗
-      (∀ v δ', semTriple δ' (Q v δ') (lift_cnt (λ _, s2) v) R) -∗
+      (∀ v δ', semTriple δ' (Q v δ') s2 R) -∗
       semTriple δ P (s1 ;; s2) R.
   Proof.
     iIntros "Hs Hk P". iApply semWP2_seq. iSpecialize ("Hs" with "P").
     iApply (semWP2_mono with "Hs"). iIntros (v1 δ1 v2 δ2) "(<- & <- & Q)".
-    iSpecialize ("Hk" with "Q"). destruct v1 as [v1|m1]; simpl; auto.
+    destruct v1 as [v1|m1]; simpl.
+    - now iSpecialize ("Hk" with "Q").
+    - now iApply semWP2_fail.
   Qed.
 
   Lemma iris_rule_stm_assertk {Γ τ} (δ : CStore Γ)
         (e1 : Exp Γ ty.bool) (e2 : Exp Γ ty.string) (k : Stm Γ τ)
-                      (P : iProp Σ) (Q : IVal τ -> CStore Γ -> iProp Σ) :
+                      (P : iProp Σ) (Q : Val τ -> CStore Γ -> iProp Σ) :
     ⊢ (⌜eval e1 δ = true⌝ -∗ semTriple δ P k Q) -∗
       (⌜eval e1 δ = false⌝ -∗ semTriple δ P (of_ival (inr (eval e2 δ))) Q) -∗
       semTriple δ P (stm_assertk e1 e2 k) Q.
@@ -930,19 +931,18 @@ Section Soundness.
   Qed.
 
   Lemma iris_rule_stm_fail {Γ} (δ : CStore Γ)
-        (τ : Ty) (s : Val ty.string) {P : iProp Σ} {Q : IVal τ -> CStore Γ -> iProp Σ} :
-    ⊢ ((P -∗ Q (inr s) δ)%I -∗ semTriple δ P (stm_fail τ s) Q).
+    (τ : Ty) (s : Val ty.string) :
+    forall {Q : Val τ -> CStore Γ -> iProp Σ},
+      ⊢ semTriple δ True (stm_fail τ s) Q.
   Proof.
-    iIntros "PQ P".
-    iApply semWP2_fail.
-    iSpecialize ("PQ" with "P").
-    iModIntro; by iFrame.
+    iIntros (Q) "_".
+    now iApply semWP2_fail.
   Qed.
 
   Lemma iris_rule_stm_read_register {Γ} (δ : CStore Γ)
         {σ : Ty} (r : 𝑹𝑬𝑮 σ) (v : Val σ) :
     ⊢ (semTriple δ (lptsreg r v) (stm_read_register r)
-         (λ v' δ', ⌜δ' = δ⌝ ∧ ⌜v' = inl v⌝ ∧ lptsreg r v)).
+         (λ v' δ', ⌜δ' = δ⌝ ∧ ⌜v' = v⌝ ∧ lptsreg r v)).
   Proof.
     iIntros "H". iApply semWP2_read_register. iExists v, v.
     iFrame. iIntros "H". repeat iSplit; auto.
@@ -954,7 +954,7 @@ Section Soundness.
                               (v : Val σ) :
         ⊢ semTriple δ (lptsreg r v) (stm_write_register r w)
             (λ v' δ',
-              ⌜δ' = δ⌝ ∧ ⌜v' = inl (eval w δ)⌝ ∧ lptsreg r (eval w δ)).
+              ⌜δ' = δ⌝ ∧ ⌜v' = eval w δ⌝ ∧ lptsreg r (eval w δ)).
   Proof.
     iIntros "H". iApply semWP2_write_register. iExists v, v.
     iFrame. iIntros "H". repeat iSplit; auto.
@@ -962,11 +962,8 @@ Section Soundness.
 
   Lemma iris_rule_stm_assign {Γ} (δ : CStore Γ)
         (x : PVar) (σ : Ty) (xIn : x∷σ ∈ Γ) (s : Stm Γ σ)
-        (P : iProp Σ) (R : IVal σ -> CStore Γ -> iProp Σ) :
-    ⊢ (semTriple δ P s (fun v δ' => R v match v with
-                                        | inl v => (@env.update _ _ _ δ' (x∷_) _ v)
-                                        | inr m => δ'
-                                        end) -∗
+        (P : iProp Σ) (R : Val σ -> CStore Γ -> iProp Σ) :
+    ⊢ (semTriple δ P s (fun v δ' => R v (@env.update _ _ _ δ' (x∷_) _ v)) -∗
            semTriple δ P (stm_assign x s) R).
   Proof.
     iIntros "Hk P". iApply semWP2_assign. iSpecialize ("Hk" with "P").
@@ -976,11 +973,11 @@ Section Soundness.
 
   Lemma iris_rule_stm_bind {Γ} (δ : CStore Γ)
         {σ τ : Ty} (s : Stm Γ σ) (k : Val σ -> Stm Γ τ)
-        (P : iProp Σ) (Q : IVal σ -> CStore Γ -> iProp Σ)
-        (R : IVal τ -> CStore Γ -> iProp Σ) :
+        (P : iProp Σ) (Q : Val σ -> CStore Γ -> iProp Σ)
+        (R : Val τ -> CStore Γ -> iProp Σ) :
         ⊢ (semTriple δ P s Q -∗
-           (∀ (v__σ : IVal σ) (δ' : CStore Γ),
-               semTriple δ' (Q v__σ δ') (lift_cnt k v__σ) R) -∗
+           (∀ (v__σ : Val σ) (δ' : CStore Γ),
+               semTriple δ' (Q v__σ δ') (k v__σ) R) -∗
            semTriple δ P (stm_bind s k) R).
   Proof.
     iIntros "trips tripk P".
@@ -988,13 +985,15 @@ Section Soundness.
     iApply semWP2_bind.
     iApply (semWP2_mono with "trips").
     iIntros (v1 δ1 v2 δ2) "(<- & <- & HR)".
-    now iApply ("tripk" with "HR").
+    destruct v1 as [v1|m1].
+    - now iApply ("tripk" with "HR").
+    - now iApply semWP2_fail.
   Qed.
 
   Lemma iris_rule_stm_call_inline_later
     {Γ} (δΓ : CStore Γ)
     {Δ σ} (f : 𝑭 Δ σ) (es : NamedEnv (Exp Γ) Δ)
-    (P : iProp Σ) (Q : IVal σ -> CStore Γ -> iProp Σ) :
+    (P : iProp Σ) (Q : Val σ -> CStore Γ -> iProp Σ) :
     ⊢ ▷ semTriple (evals es δΓ) P (FunDef f) (fun v _ => Q v δΓ) -∗
       semTriple δΓ P (stm_call f es) Q.
   Proof.
@@ -1006,7 +1005,7 @@ Section Soundness.
   Lemma iris_rule_stm_call_inline
     {Γ} (δΓ : CStore Γ)
     {Δ σ} (f : 𝑭 Δ σ) (es : NamedEnv (Exp Γ) Δ)
-    (P : iProp Σ) (Q : IVal σ -> CStore Γ -> iProp Σ) :
+    (P : iProp Σ) (Q : Val σ -> CStore Γ -> iProp Σ) :
     ⊢ semTriple (evals es δΓ) P (FunDef f) (fun v _ => Q v δΓ) -∗
       semTriple δΓ P (stm_call f es) Q.
   Proof.
@@ -1015,7 +1014,7 @@ Section Soundness.
 
   Lemma iris_rule_stm_debugk
     {Γ τ} (δ : CStore Γ) (k : Stm Γ τ)
-    (P : iProp Σ) (Q : IVal τ -> CStore Γ -> iProp Σ) :
+    (P : iProp Σ) (Q : Val τ -> CStore Γ -> iProp Σ) :
     ⊢ (semTriple δ P k Q -∗
        semTriple δ P (stm_debugk k) Q).
   Proof.
@@ -1023,7 +1022,7 @@ Section Soundness.
   Qed.
 
   Lemma iris_rule_noop {Γ σ} {δ : CStore Γ}
-        {P} {Q : IVal σ -> CStore Γ -> iProp Σ} {s : Stm Γ σ} :
+        {P} {Q : Val σ -> CStore Γ -> iProp Σ} {s : Stm Γ σ} :
     stm_to_val s = None ->
     (forall {s' γ γ' μ μ' δ'}, ⟨ γ, μ, δ, s ⟩ ---> ⟨ γ', μ', δ', s' ⟩ ->
                             (γ' = γ) /\ (μ' = μ) /\ (δ' = δ) /\
@@ -1040,42 +1039,38 @@ Section Soundness.
     - do 3 iModIntro. iMod "Hclose" as "_".
       iFrame. iModIntro. iApply semWP_val.
       iExists γ21, μ21, δ, (of_ival (inl v)), (inl v).
-      iMod ("HPQ" $! (inl v) with "HP") as "$". repeat iModIntro.
+      iMod ("HPQ" $! v with "HP") as "$". repeat iModIntro.
       iFrame "Hreg2 Hmem2". repeat iSplit; auto. iPureIntro. eapply step_trans.
       apply Hs2. apply step_refl.
     - do 3 iModIntro. iMod "Hclose" as "_". iFrame "Hres1".
-      iModIntro. iApply semWP_fail. iMod ("HPQ" $! (inr msg) with "HP") as "HQ".
+      iModIntro. iApply semWP_fail.
       repeat iModIntro. iExists γ21, μ21, δ, (of_ival (inr msg)), (inr msg).
-      iFrame "Hreg2 Hmem2 HQ". repeat iSplit; auto. iPureIntro.
+      iFrame "Hreg2 Hmem2". repeat iSplit; auto. iPureIntro.
       eapply step_trans. apply Hs2. simpl. apply step_refl.
   Qed.
 
   Lemma iris_rule_stm_pattern_match {Γ τ σ} (δΓ : CStore Γ)
     (s : Stm Γ σ) (pat : Pattern σ)
     (rhs : ∀ pc : PatternCase pat, Stm (Γ ▻▻ PatternCaseCtx pc) τ)
-    (P : iProp Σ) (Q : IVal σ → CStore Γ → iProp Σ) (R : IVal τ → CStore Γ → iProp Σ) :
+    (P : iProp Σ) (Q : Val σ → CStore Γ → iProp Σ) (R : Val τ → CStore Γ → iProp Σ) :
     ⊢ semTriple δΓ P s Q -∗
-      (∀ v δΓ1,
-          match v with
-          | inl v =>
+      (∀ (v : Val σ) δΓ1,
               ∀ pc δpc,
-                semTriple (δΓ1 ►► δpc) (Q (inl (pattern_match_val_reverse pat pc δpc)) δΓ1) (rhs pc)
-                  (λ vτ (δ' : CStore (Γ ▻▻ PatternCaseCtx pc)), R vτ (env.drop (PatternCaseCtx pc) δ'))
-          | inr m => semTriple δΓ1 (Q v δΓ1) (of_ival (inr m)) R
-          end) -∗
+                semTriple (δΓ1 ►► δpc) (Q (pattern_match_val_reverse pat pc δpc) δΓ1) (rhs pc)
+                  (λ vτ (δ' : CStore (Γ ▻▻ PatternCaseCtx pc)), R vτ (env.drop (PatternCaseCtx pc) δ'))) -∗
       semTriple δΓ P (stm_pattern_match s pat rhs) R.
   Proof.
     iIntros "Hs Hk P". iApply semWP2_pattern_match. iSpecialize ("Hs" with "P").
     iApply (semWP2_mono with "Hs"). iIntros (v1 δ1 v2 δ2) "(<- & <- & Q)".
     destruct v1 as [v1|m1].
     - destruct (pattern_match_val pat v1) as [pc δpc] eqn:Ev1.
-      iSpecialize ("Hk" $! (inl v1) δ1 pc δpc with "[Q]").
+      iSpecialize ("Hk" $! v1 δ1 pc δpc with "[Q]").
       { change (pattern_match_val_reverse pat pc δpc) with
           (pattern_match_val_reverse' pat (existT pc δpc)).
         rewrite <- Ev1. now rewrite pattern_match_val_inverse_left. }
       iApply (semWP2_mono with "Hk"). iIntros (? ? ? ?) "(<- & <- & R)".
       now iFrame "R".
-    - now iSpecialize ("Hk" $! (inr m1) with "Q").
+    - now iApply semWP2_fail.
   Qed.
 
   Definition ValidContractSemCurried {Δ σ} (body : Stm Δ σ) (contract : SepContract Δ σ) : iProp Σ :=
@@ -1083,11 +1078,7 @@ Section Soundness.
     | MkSepContract _ _ ctxΣ θΔ pre result post =>
       Sep.Logic.Forall (fun (ι : Valuation ctxΣ) =>
         semTriple (inst θΔ ι) (asn.interpret pre ι) body
-          (λ v δ,
-            match v with
-            | inl v => asn.interpret post (env.snoc ι (result∷σ) v)
-            | inr m => True%I (* TODO: we can do something better here *)
-            end))
+                  (fun v δ' => asn.interpret post (env.snoc ι (result∷σ) v)))
     end.
 
   Definition ValidContractSem {Δ σ} (body : Stm Δ σ) (contract : SepContract Δ σ) : iProp Σ :=
@@ -1095,11 +1086,7 @@ Section Soundness.
     | MkSepContract _ _ ctxΣ θΔ pre result post =>
       ∀ (ι : Valuation ctxΣ),
         semTriple (inst θΔ ι) (asn.interpret pre ι) body
-          (λ v δ,
-            match v with
-            | inl v => asn.interpret post (env.snoc ι (result∷σ) v)
-            | inr m => True%I (* TODO: we can do something better here *)
-            end)
+          (λ v δ, asn.interpret post (env.snoc ι (result∷σ) v))
     end.
 
   Definition ValidContractForeign {Δ τ} (contract : SepContract Δ τ) (f : 𝑭𝑿 Δ τ) : Prop :=
@@ -1109,11 +1096,7 @@ Section Soundness.
         forall (ι : Valuation Σ'),
         evals es δ = inst θΔ ι ->
         ⊢ semTriple δ (asn.interpret req ι) (stm_foreign f es)
-          (λ v δ',
-            match v with
-            | inl v => asn.interpret ens (env.snoc ι (result∷τ) v) ∗ bi_pure (δ' = δ)
-            | inr m => True%I (* TODO: we can do something better here *)
-            end)
+          (λ v δ', asn.interpret ens (env.snoc ι (result∷τ) v) ∗ bi_pure (δ' = δ))
       end.
 
   Definition valid_contract_curry {Δ σ} (body : Stm Δ σ) (contract : SepContract Δ σ) :
